spec/crypto/pow2.s.dfy
@@ -19,17 +19,32 @@ module pow2_s {
         pow2_t_cons(Pow(2, exp), exp)
     }
 
-    lemma pow2_basics(n: pow2_t)
+    lemma pow2_basics_lemma(n: pow2_t)
         ensures n.exp == 0 <==> n.full == 1
         ensures n.exp == 1 <==> n.full == 2
         ensures n.exp != 0 ==> n.full % 2 == 0
         ensures n.full >= 1
     {
-        // LemmaPowStrictlyIncreasesAuto();
-        assume n.exp == 1 <==> n.full == 2;
-        LemmaPowPositiveAuto();
         reveal Pow();
         reveal Pow2();
+        if n.full == 2 && n.exp != 1{
+            assert n.exp != 0;
+            assert n.exp > 1;
+            LemmaPowStrictlyIncreases(2, 1, n.exp);
+        }
+        LemmaPowPositiveAuto();
+    }
+
+    lemma pow2_increases_lemma(n: pow2_t, n': pow2_t)
+        ensures n.exp < n'.exp <==> n.full < n'.full;
+    {
+        reveal Pow2();
+        if n.exp < n'.exp {
+            LemmaPowStrictlyIncreases(2, n.exp, n'.exp);
+        }
+        if n.full < n'.full {
+            LemmaPowStrictlyIncreasesConverse(2, n.exp, n'.exp);
+        }
     }
 
     lemma pow2_half_value_lemma(n: pow2_t, n': pow2_t_raw)
@@ -39,7 +54,7 @@ module pow2_s {
         ensures n'.full * 2 == n.full
         ensures n'.full == Pow2(n'.exp);
     {
-        pow2_basics(n);
+        pow2_basics_lemma(n);
 
         calc == {
             n'.full;
@@ -61,7 +76,7 @@ module pow2_s {
         ensures n.full % 2 == 0;
         ensures n'.full == n.full / 2;
     {
-        pow2_basics(n);
+        pow2_basics_lemma(n);
         assert n.exp - 1 >= 0;
         var m := pow2_t_cons(n.full / 2, n.exp - 1);
         pow2_half_value_lemma(n, m);
@@ -72,7 +87,7 @@ module pow2_s {
         ensures n'.exp == n.exp + 1;
         ensures n'.full == n.full * 2;
     {
-        pow2_basics(n);
+        pow2_basics_lemma(n);
         reveal Pow2();
         reveal Pow();
         var m := pow2_t_cons(n.full * 2, n.exp + 1);
@@ -94,8 +109,8 @@ module pow2_s {
         ensures n.full % m.full == 0;
         ensures n.full == n'.full * m.full;
     {
-        pow2_basics(m);
-        pow2_basics(n);
+        pow2_basics_lemma(m);
+        pow2_basics_lemma(n);
         LemmaPowSubtracts(2, m.exp, n.exp);
         reveal Pow2();
         var a := pow2_t_cons(n.full / m.full, n.exp - m.exp);
